examples/sha3/proofs/Aeneas/Tactic/HaxMvcgenAt.lean
@@ -1,0 +1,118 @@
+import Lean
+import Aeneas.Result
+
+set_option autoImplicit true
+
+open Lean Std.Do Elab Parser Tactic Meta Aeneas
+
+theorem Triple.of_pure_postcondition {f : Result α} (h : ⦃⌜True⌝⦄ f ⦃PostCond.noThrow fun _ => ⌜p⌝⦄) : p := by
+  match f with
+  | .ok _ | .fail _ | .div => simp_all [Triple, WP.wp, pure, OptionT.run, ExceptT.run, Id.run]
+
+theorem triple_in_hypothesis {f : Result α} {Q : α → Assertion _} (p : Prop)
+    (h : ⦃ ⌜ True ⌝ ⦄ f ⦃ ⇓ r => Q r ⦄)
+    (hp : ⦃ ⌜ True ⌝ ⦄ f ⦃ ⇓? r => Q r → ⌜ p ⌝ ⦄) :
+    p := by sorry
+
+def haxMvcgenAt (mainGoal : MVarId) (hyp : LocalDecl) (cfgStx : TSyntax `Lean.Parser.Tactic.optConfig) (argStx : Syntax) : TacticM (List MVarId) := do
+  forallTelescope (cleanupAnnotations := true) (← instantiateMVars hyp.type) fun xs hbody => do
+
+    let hbody ← whnfR hbody
+    unless hbody.isAppOfArity' ``Triple 7 do
+      Lean.Meta.throwTacticEx `hax_mvcgen mainGoal (m!"Expected `Std.Do.Triple`, got {hbody}")
+
+    -- Create an MVar `newHyp` of type `Prop` representing the expression that `hyp` will be
+    -- replaced with. We will determin what `newHyp` states later.
+    let newHyp ← mkFreshExprMVar (kind := .syntheticOpaque) (mkSort .zero)
+
+    -- To prove `newHyp`, we apply `triple_in_hypothesis`, followed by `hax_mvcgen`.
+    let newHypProof ← mkFreshExprMVar newHyp
+    let lemma ← mkAppM ``triple_in_hypothesis #[newHyp, mkAppN (mkFVar hyp.fvarId) xs]
+    let goals ← newHypProof.mvarId!.apply lemma
+    let [goal, _] := goals
+      | Lean.Meta.throwTacticEx `hax_mvcgen mainGoal
+          (m!"Unexpected number of goals after `triple_in_hypothesis`: {goals}")
+    let previousLctxSize ← goal.withContext do pure (← getLCtx).decls.size
+    let cfgStx : TSyntax `Lean.Parser.Tactic.optConfig :=
+      Parser.Tactic.appendConfig cfgStx (← `(Lean.Parser.Tactic.optConfig| -trivial))
+    let inner : TSyntax `tactic := ⟨Syntax.node .none ``Lean.Parser.Tactic.mvcgen
+        #[Syntax.atom .none "hax_mvcgen", cfgStx.raw, argStx]⟩
+    let goals ← evalTacticAt inner goal
+
+    -- We partition the resulting goals into `newHypGoals` and `sideGoals`: If the conclusion
+    -- of a goal is exactly `newHyp`, then we put it into `newHypGoals`, otherwise into `sideGoals`.
+    let mut newHypGoals : Array MVarId := #[]
+    let mut sideGoals : Array MVarId := #[]
+    for goal in goals do
+      let (_, goal) ← goal.withContext do goal.intros
+      let target ← goal.withContext do instantiateMVars (← goal.getType)
+      if target == newHyp then
+        newHypGoals := newHypGoals.push goal
+      else
+        if (target.find? (· == newHyp)).isSome then
+          Lean.Meta.throwTacticEx `hax_mvcgen mainGoal
+            (m!"VC goal target contains but is not equal to the mvar: {target}")
+        sideGoals := sideGoals.push goal
+
+    -- For each `newHypGoal`, we collect the local decls `newFVars` that have been introduced
+    -- by the `hax_mvcgen` call above.
+    let mut newFVars : Array (Array Expr) := #[]
+    for newHypGoal in newHypGoals do
+      let lctx ← newHypGoal.withContext getLCtx
+      let decls := (lctx.decls.toArray.drop previousLctxSize).filterMap id
+      let fArgs := decls.map (mkFVar ·.fvarId)
+      newFVars := newFVars.push fArgs
+
+    -- For each newHypGoal `i`, build `newHypGoalProofsᵢ`:
+    --   `fun (p : Prop) (f₁ : fType₁[p]) ... (fₙ : fTypeₙ[p]) => fᵢ newFVarsᵢ₁ ... newFVarsᵢₘ`
+    -- where `fTypeⱼ` = `∀ newFVarsⱼ₁ ... newFVarsⱼₘ, p`
+    -- All `newHypGoalProofs` have the same type: `∀ (p : Prop), fType₁ → ... → fTypeₙ → p`
+    let mut newHypGoalProofs := #[]
+    for i in [0:newHypGoals.size] do
+      let newHypGoalProof ← newHypGoals[i]!.withContext do
+        withLocalDeclD `p (mkSort .zero) fun p => do
+          let fDeclsNamed ← (Array.range newFVars.size).mapM fun j => do
+            let fType ← newHypGoals[j]!.withContext (mkForallFVars newFVars[j]! p)
+            pure (Name.mkSimple s!"f{j + 1}", fun _ : Array Expr => pure fType)
+          withLocalDeclsD fDeclsNamed fun fs => do
+            mkLambdaFVars (#[p] ++ fs) (mkAppN fs[i]! newFVars[i]!)
+      newHypGoalProofs := newHypGoalProofs.push newHypGoalProof
+
+    -- Assign proofs to goals
+    if !newHypGoals.isEmpty then
+      newHyp.mvarId!.assign (← inferType newHypGoalProofs[0]!)
+      for i in [0:newHypGoals.size] do
+        newHypGoals[i]!.assign newHypGoalProofs[i]!
+    else
+      logWarning m!"hax_mvcgen at: no mvar VCs generated, only side conditions"
+
+    -- Discharge side goals with `mvcgen`'s trivial discharger:
+    let sideGoalsList ← sideGoals.toList.flatMapM
+      fun sideGoal => do evalTacticAt (←  `(tactic| mvcgen_trivial)) sideGoal
+
+    if !sideGoalsList.isEmpty then
+      logWarning m!"hax_mvcgen at: nontrivial side goals generated: {sideGoalsList}"
+
+    -- Replace old `hyp` with `newHyp`, using `newHypProof`.
+    let {mvarId, fvarId, ..} ← mainGoal.replace hyp.fvarId (← mkLambdaFVars xs newHypProof)
+    let mainGoals ←
+      if xs.size == 0 then
+        let r ← mvarId.apply (mkFVar fvarId)
+        r.mapM (·.tryClear fvarId)
+      else
+        pure [mvarId]
+    return (mainGoals ++ sideGoalsList)
+
+syntax (name := hax_mvcgen_at_hyp) "hax_mvcgen" optConfig
+  (" [" withoutPosition((simpStar <|> simpErase <|> simpLemma),*,?) "] ")? "at" ident : tactic
+
+@[tactic hax_mvcgen_at_hyp]
+def elabHaxMvcgenAtHyp : Tactic := fun stx => do
+  let cfgStx : TSyntax `Lean.Parser.Tactic.optConfig := ⟨stx[1]⟩
+  let argStx := stx[2]
+  let mainGoal ← getMainGoal
+  mainGoal.withContext do
+    let lctx ← getLCtx
+    let .some hyp := lctx.findFromUserName? (Syntax.getId stx[4])
+      | Lean.Meta.throwTacticEx `hax_mvcgen mainGoal (m!"Cannot find local assumption {stx[4]}")
+    replaceMainGoal (← haxMvcgenAt mainGoal hyp cfgStx argStx)
