examples/sha3/proofs/Sha3/Equivalence.lean
@@ -6,9 +6,15 @@ namespace sha3
 #check reference.iota
 
 -- The real implementaion
-#check KeccakState.iota
+#check iota
 
-theorem KeccakState.iota_spec :
-  ⦃ ⌜ True ⌝ ⦄
-  KeccakState.iota
-  ⦃ ⇓ r => ⌜ ⌝ ⦄
+open Std.Do Aeneas
+set_option mvcgen.warning false
+
+theorem iota_spec
+  (st : KeccakState U64.Insts.Sha3KeccakItem1) (i : Std.Usize)
+  (h : (_requires_iota st i).holds):
+    ⦃ ⌜ True ⌝ ⦄
+    iota st i
+    ⦃ ⇓ r => ⌜ (_ensures_iota st i r).holds ⌝ ⦄ := by
+  hax_mvcgen [iota, KeccakState.iota, _requires_iota]
